LeanOS.lean
@@ -13,6 +13,7 @@ import LeanOS.IPCSyscall
 import LeanOS.Interrupt
 import LeanOS.InterruptEntry
 import LeanOS.PrivilegeEntryStack
+import LeanOS.PrivilegeEntryControl
 import LeanOS.Example
 import LeanOS.FrameAllocator
 import LeanOS.FrameBudget
